src/LibListExec.v
@@ -6,13 +6,11 @@
 Set Implicit Arguments.
 Generalizable Variables A B.
 From TLC Require Import LibTactics LibReflect.
-From TLC Require Export LibList.
+From TLC Require Export LibNat LibList.
 
 
 (* ---------------------------------------------------------------------- *)
 (* ** Autorewrite *)
-
-Module RewListExec.
 
 Tactic Notation "rew_list_exec" :=
   autorewrite with rew_list_exec.
@@ -21,8 +19,6 @@ Tactic Notation "rew_list_exec" "in" "*" :=
   (* autorewrite with rew_list_exec in *. *)
 Tactic Notation "rew_list_exec" "in" hyp(H) :=
   autorewrite with rew_list_exec in H.
-
-End RewListExec.
 
 
 (* ---------------------------------------------------------------------- *)
@@ -50,8 +46,7 @@ Proof.
   intros. destruct l; simpl; rew_bool_eq; auto_false.
 Qed.
 
-#[global]
-Hint Rewrite is_nil_eq is_not_nil_eq : rew_list_exec.
+#[global] Hint Rewrite is_nil_eq is_not_nil_eq : rew_list_exec.
 
 
 (* ---------------------------------------------------------------------- *)
@@ -64,8 +59,7 @@ Lemma length_eq :
   length = LibList.length.
 Proof using. extens ;=> A l. induction l; simpl; rew_list; auto. Qed.
 
-#[global]
-Hint Rewrite length_eq : rew_list_exec.
+#[global] Hint Rewrite length_eq : rew_list_exec.
 
 
 (* ---------------------------------------------------------------------- *)
@@ -80,8 +74,7 @@ Proof using.
   extens ;=> A L1 L2. induction L1; simpl; rew_list; congruence.
 Qed.
 
-#[global]
-Hint Rewrite app_eq : rew_list_exec.
+#[global] Hint Rewrite app_eq : rew_list_exec.
 
 
 (* ---------------------------------------------------------------------- *)
@@ -97,22 +90,7 @@ Proof using.
   { rewrite IHL. rewrite <- app_eq. unfold app. fequals. }
 Qed.
 
-#[global]
-Hint Rewrite rev_eq : rew_list_exec.
-
-
-(* ---------------------------------------------------------------------- *)
-(* ** [fold_right] *)
-
-Definition fold_right : forall A B, (B->A->A) -> A -> list B -> A :=
-  @List.fold_right.
-
-Lemma fold_right_eq : forall A B (f:B->A->A) (a:A) (l:list B),
-  fold_right f a l = LibList.fold_right f a l.
-Proof using. intros. induction l; simpl; rew_listx; fequals. Qed.
-
-#[global]
-Hint Rewrite fold_right_eq : rew_list_exec.
+#[global] Hint Rewrite rev_eq : rew_list_exec.
 
 
 (* ---------------------------------------------------------------------- *)
@@ -127,8 +105,183 @@ Proof using.
   extens ;=> A B f L. induction L; simpl; rew_listx; congruence.
 Qed.
 
-#[global]
-Hint Rewrite map_eq : rew_list_exec.
+#[global] Hint Rewrite map_eq : rew_list_exec.
+
+(* ---------------------------------------------------------------------- *)
+(* ** [mem] *)
+
+Fixpoint mem A (cmp:A->A->bool) (x:A) (l:list A) : bool :=
+  match l with
+  | nil => false
+  | y::l' => cmp x y || mem cmp x l'
+  end.
+
+Lemma mem_eq : forall A (cmp:A->A->bool) x l,
+  is_beq cmp ->
+  mem cmp x l = isTrue (LibList.mem x l).
+Proof using.
+  introv M. induction l as [|y l']; simpl; rew_listx; rew_isTrue; fequals.
+Qed.
+
+#[global] Hint Rewrite mem_eq : rew_list_exec.
+
+
+(* ---------------------------------------------------------------------- *)
+(** ** [concat] *)
+
+Definition concat A (m:list (list A)) : list A :=
+  fold_right (@app A) (@nil A) m.
+
+Transparent LibList.concat.
+Lemma concat_eq :
+  concat = LibList.concat.
+Proof using.
+  unfold concat. rew_list_exec. unfold LibList.concat. rew_list_exec. auto.
+Qed.
+
+#[global] Hint Rewrite concat_eq : rew_list_exec.
+
+
+(* ---------------------------------------------------------------------- *)
+(** ** [filter] *)
+
+Definition filter A (p:A->bool) (l:list A) : list A :=
+  fold_right (fun x acc => if p x then x::acc else acc) (@nil A) l.
+
+Lemma filter_eq : forall A (p:A->bool) (P:A->Prop) l,
+  isTrue_pred p P ->
+  filter p l = LibList.filter P l.
+Proof using.
+  Local Transparent LibList.filter.
+  introv E. unfold filter, LibList.filter. rew_list_exec. 
+  fequals. extens. intros. rewrite E. rewrite* if_isTrue.
+Qed.
+
+#[global] Hint Rewrite filter_eq : rew_list_exec.
+
+
+(* ---------------------------------------------------------------------- *)
+(** ** [remove] *)
+
+Definition remove A (cmp:A->A->bool) (a:A) (l:list A) : list A :=
+  filter (fun x => neg (cmp a x)) l.
+
+Lemma remove_eq : forall A (cmp:A->A->bool) (a:A) (l:list A),
+  is_beq cmp ->
+  remove cmp a l = LibList.remove a l.
+Proof using.
+  Local Transparent LibList.remove.
+  introv E. unfold remove, LibList.remove.
+  rewrites* (>> filter_eq (<> a)).
+  { intros x. rewrite E. rew_isTrue. fequals. rew_bool_eq*. }
+Qed.
+
+#[global] Hint Rewrite remove_eq : rew_list_exec.
+
+
+(* ---------------------------------------------------------------------- *)
+(* ** [noduplicates] *)
+
+Fixpoint noduplicates A (cmp:A->A->bool) (l:list A) : bool :=
+  match l with
+  | nil => true
+  | x::l' => neg (mem cmp x l') && noduplicates cmp l'
+  end.
+
+Lemma noduplicates_eq : forall A (cmp:A->A->bool) (l:list A),
+  is_beq cmp ->
+  noduplicates cmp l = isTrue (LibList.noduplicates l).
+Proof using.
+  introv E. extens. induction l as [|x l']; simpl; rew_listx; rew_bool_eq in *.
+  { autos*. }
+  { rewrite* mem_eq. rew_bool_eq. iff (M1&M2); splits*. }
+Qed.
+
+#[global] Hint Rewrite noduplicates_eq : rew_list_exec.
+
+
+(* ---------------------------------------------------------------------- *)
+(* ** [remove_duplicates] *)
+
+Fixpoint remove_duplicates A (cmp:A->A->bool) (l:list A) : list A :=
+  match l with
+  | nil => nil
+  | x::l' => x :: (remove cmp x (remove_duplicates cmp l'))
+  end.
+
+Lemma remove_duplicates_eq : forall A (cmp:A->A->bool) (l:list A),
+  is_beq cmp ->
+  remove_duplicates cmp l = LibList.remove_duplicates l.
+Proof using.
+  Local Transparent LibList.remove_duplicates.
+  introv E. induction l as [|x l']; simpl; fequals.
+  rewrite* remove_eq. congruence.
+Qed.
+
+#[global] Hint Rewrite remove_duplicates_eq : rew_list_exec.
+
+
+(* ---------------------------------------------------------------------- *)
+(* ** [Forall] *)
+
+Fixpoint Forall A (p:A->bool) (l:list A) : bool :=
+  match l with
+  | nil => true
+  | x::l' => p x && Forall p l'
+  end.
+
+Lemma Forall_eq : forall A (p:A->bool) (P:A->Prop) l,
+  isTrue_pred p P ->
+  Forall p l = isTrue (LibList.Forall P l).
+Proof using.
+  introv E. extens. induction l as [|x l']; simpl; rew_listx in *; rew_bool_eq in *.
+  { iff*. }
+  { rewrite E. rew_bool_eq. iff*. }
+Qed.
+
+#[global] Hint Rewrite Forall_eq : rew_list_exec.
+
+
+(* ---------------------------------------------------------------------- *)
+(* ** [Exists] *)
+
+Fixpoint Exists A (p:A->bool) (l:list A) : bool :=
+  match l with
+  | nil => false
+  | x::l' => p x || Exists p l'
+  end.
+
+Lemma Exists_eq : forall A (p:A->bool) (P:A->Prop) l,
+  isTrue_pred p P ->
+  Exists p l = isTrue (LibList.Exists P l).
+Proof using.
+  introv E. extens. induction l as [|x l']; simpl; rew_listx in *; rew_bool_eq in *.
+  { iff*. }
+  { rewrite E. rew_bool_eq. iff*. }
+Qed.
+
+#[global] Hint Rewrite Exists_eq : rew_list_exec.
+
+
+(* ---------------------------------------------------------------------- *)
+(* ** [Count] *)
+
+Fixpoint count A (p:A->bool) (l:list A) : nat :=
+  match l with
+  | nil => 0%nat
+  | x::l' => if p x then S (count p l') else count p l'
+  end.
+
+Lemma count_eq : forall A (p:A->bool) (P:A->Prop) l,
+  isTrue_pred p P ->
+  count p l = LibList.count P l.
+Proof using.
+  introv E. induction l as [|x l']; simpl; rew_listx.
+  { auto. }
+  { rewrite IHl'. rewrite E. do 2 case_if; try nat_math. }
+Qed.
+
+#[global] Hint Rewrite count_eq : rew_list_exec.
 
 
 (* ---------------------------------------------------------------------- *)
@@ -147,23 +300,19 @@ Proof using. (* --LATER: conduct proof using list2_ind *)
   { rew_list in E. rew_listx. simpl. fequals~. }
 Qed.
 
-#[global]
-Hint Rewrite combine_eq : rew_list_exec.
+#[global] Hint Rewrite combine_eq : rew_list_exec.
 
 
 (* ---------------------------------------------------------------------- *)
-(* ** [mem] *)
+(* ** [fold_right] *)
 
-Fixpoint mem A (cmp:A->A->bool) (x:A) (l:list A) : bool :=
-  match l with
-  | nil => false
-  | y::l' => cmp x y || mem cmp x l'
-  end.
+(** [LibList.fold_right] computes well. Here, we prove that it matches 
+    Coq's standard library [fold_right]. *)
 
-Lemma mem_exec_eq : forall A (cmp:A->A->bool) x l,
-  is_beq cmp ->
-  mem cmp x l = isTrue (LibList.mem x l).
-Proof using.
-  introv M. induction l as [|y l']; simpl; rew_listx; rew_isTrue; fequals.
-Qed.
+Lemma fold_right_eq : forall A B,
+  @List.fold_right B A = @LibList.fold_right A B.
+Proof using. extens. intros a b l. induction l; simpl; rew_listx; fequals. Qed.
+
+#[global] Hint Rewrite fold_right_eq : rew_list_exec.
+
 
